lean/AxiomsCheck.lean
@@ -1,5 +1,9 @@
 import Correctness
+import Proposals
 #print axioms Redgrep.nullable_correct
 #print axioms Redgrep.lang_deriv
 #print axioms Redgrep.deriv_correct
 #print axioms Redgrep.matchRE_correct
+#print axioms Redgrep.matchW_correct
+#eval Redgrep.matchRE (.invHom (fun c => [c, c]) (.rep (.sym (fun c => c == 'a')))) ['a', 'a']
+#eval Redgrep.matchRE (.invHom (fun _ => []) .eps) ['x', 'y']
